\begin{solution}{normal}
The tire does not exchange any heat with its surroundings which means that it undergoes an adiabatic expansion/compression. Since we are relating two state variables $p$ and $T$, we use the relation
\[p^{1 - \gamma}T^{\gamma} = \text{const.}\]Substituting both final and initial variables shows us
\[p_0^{1 - \gamma} T_0^{\gamma} = p_f^{1 - \gamma} T_f^{\gamma}\implies T_f = T_0 \left(\frac{p_f}{p_0}\right)^{\frac{\gamma - 1}{\gamma}} = T_0 \left(\frac{p_0 + p_1}{p_0}\right)^{\frac{\gamma - 1}{\gamma}} = 3^{\frac{\gamma - 1}{\gamma}} T_0\approx 400\;\mathrm{K}.\]
\end{solution}