\begin{solution}{normal}
The smoke rises until it's density becomes the same as the density of the air around it. From problem 69 and 70, note that 
\[\frac{\text{d}T}{T} = (1 - \gamma^{-1}) \frac{\text{d}p}{p}\implies \Delta T = T (1 - \gamma^{-1}) \frac{\Delta p}{p}.\]
The change in pressure is given by $\Delta p = \rho gh$ and since $\rho = p\mu/RT$ from the ideal gas law, we get 
\[\Delta p = \frac{p \mu}{RT} gh\]
also note that 
\[\gamma^{-1} = \frac{c_V}{c_p} = \frac{c_V}{c_V + R}\]
which means that 
\[\Delta T = \frac{R}{c_V + R}\frac{\mu gh}{R}.\]
Rearranging to solve for $h$ tells us that 
\[h = \frac{\Delta T R (c_V + R)}{\mu g}.\]
\end{solution}