\begin{solution}{normal}
We see from the 3 dimensional distance formula that the distance between $(t_1, x_1, y_1, z_1)$ and $(t_2, x_2, y_2, z_2)$ is 
\[d = \sqrt{(x_2-x_1)^2 + (y_2 - y_1)^2 + (z_2 - z_1)^2}\]
We also know that from fact 1 that
\[t = t_2 - t_1 = \gamma\tau.\]
Squaring both sides gives us 
\begin{align*}
t^2 &= \frac{\gamma^2}{1-v^2/c^2}\\
t^2 (c^2 - v^2) &= c^2\tau^2 \implies c^2t^2 - v^2t^2 = c^2\tau^2
\end{align*}
We know from basic kinematic relations that $v= dt\implies d^2 = v^2t^2$, therefore, by substituting this into our expression we find that 
\begin{align*}
c^2t^2 &- d^2= c^2\tau^2\\
c^2\tau^2&= c^2t^2 - (x_2-x_1)^2 - (y_2 - y_1)^2 - (z_2 - z_1)^2
\end{align*}
Substituting our first expression for $t$ gives 
\[\boxed{c^2\tau^2= c^2(t_2 - t_1)^2 - (x_2-x_1)^2 - (y_2 - y_1)^2 - (z_2 - z_1)^2}\]
\end{solution}