\begin{solution}{normal}
We see that in the imaginary plane, 
\begin{align*}
e^\varphi &= \cos\alpha + i\sin\alpha\\
e^{-\varphi} &= \cos\alpha - i\sin\alpha
\end{align*}
In hyperbolic geometry, 
\[\tan\varphi = \frac{\sinh\varphi}{\cosh\varphi}= \frac{e^\alpha - e^{-\alpha}}{e^\alpha + e^{-\alpha}}= \frac{\cos\alpha + i\sin\alpha - \cos\alpha + i\sin\alpha}{\cos\alpha + i\sin\alpha + \cos\alpha - i\sin\alpha}= \frac{2i\sin\alpha}{2\cos\alpha}\]
From fact 7, we then find that 
\[\tanh\varphi = \frac{\beta\gamma}{\gamma} = \beta.\]
In hyperbolic geometry, 
\[\sinh\varphi = \frac{e^\varphi - e^{-\varphi}}{2} = \frac{\cos\alpha + i\sin\alpha - \cos\alpha + i\sin\alpha}{2}.\]
From fact 7, we then find that 
\[\sinh\varphi = i\sin\alpha = \beta\gamma.\]
In hyperbolic geometry, 
\[\cosh\varphi = \frac{e^\varphi + e^{-\varphi}}{2} = \frac{\cos\alpha + i\sin\alpha + \cos\alpha - i\sin\alpha}{2}\]
From fact 7, we find that 
\[\cosh\varphi = \cos\alpha = \gamma\]
\end{solution}