\begin{solution}{normal}
From fact 21, we see that the kinetic energy is given by 
\[E_k = (\gamma - 1)mc^2.\]
Replacing $\gamma$ with $\frac{1}{\sqrt{1-v^2/c^2}}$ gives us 
\[E_k = \left(\frac{1}{\sqrt{1-v^2/c^2}} - 1\right)mc^2\]
Now, we use a taylor series approximation. We note that when $x\ll 1$, then 
\[(1 + x)^n = 1+nx\]
holds true. Using this fact for $\gamma$ gives us 
\[\left(1+\left(-\frac{v^2}{c^2}\right)\right)^{-1/2} = 1 + \frac{v^2}{2c^2}.\]
Substituting back in lets us get 
\[E_k = \left(\left(1 + \frac{v^2}{2c^2}\right) - 1\right)mc^2 \equiv \frac{1}{2}mv^2\]

\end{solution}