\begin{solution}{normal}
We know that from fact 1 that
\[t = t_2 - t_1 = \gamma\tau.\]Squaring both sides gives us
\begin{align*}
t^2 &= \frac{\gamma^2}{1-v^2/c^2}\\
t^2 (c^2 - v^2) &= c^2\tau^2 \implies c^2t^2 - v^2t^2 = c^2\tau^2
\end{align*}
We know from basic kinematic relations that $v= dt\implies d^2 = v^2t^2$, therefore, by substituting this into our expression (with $d^2 = 4\pi r^2$) we find that
\[c^2t^2-4\pi r^2 = c^2\tau^2\implies \boxed{r=\frac{c\sqrt{t^2 - \tau^2}}{2\pi}}\]
\end{solution}