\begin{solution}{normal}
According to idea 18,  we “cut off” the first period of the infinite chain ; the remaining part is equivalent to the original circuit of (yet unknown) resistance $R$. 
\begin{center}
\begin{tikzpicture}[transform shape, scale=1.5, thick]
\ctikzset{label/align = smart}
\draw (0, 0) to [open, *-] (0, 1);
\draw (0, 2) to [open, *-] (0, 0);
\draw (0, 0) -- (2, 0) to [R, l=$R_2$] (2, 2) to [R, l=$R_1$] (0, 2);
\draw (2, 2) -- (3, 2) to [R, l=$R$, blue] (3, 0) -- (2, 0);
\end{tikzpicture}
\end{center}
Because of that, we can write equality
\[R = R_1 + \frac{R R_2}{R + R_2}\]
which upon cross multiplying, gives us the equation 
\[R^2 - RR_1 - R_1 R = 0\implies R = \frac{R_1}{2}\left(1 + \sqrt{1 + \frac{4R_2}{R_1}}\right)\]
by the quadratic equation.
\end{solution}