\begin{solution}{hard}
Note that
\[dk = \frac {ds}{L(t)} = \frac {vdt}{L+ut}.\]
Integrating both sides gives us
\[\int_{0}^{1} dk = \int_{0}^{T} \frac {vdt}{L+ut}\] 
Using a $s$ substitution $s = L+ut \Rightarrow dx = udt$ and rearranging the integral gives us 
\begin{align*}
1 = \frac {v}{u} \int_{0}^{T} \frac {dx}{s} \implies \frac {u}{v} &= \ln(ut+L)\mid_{0}^{T}\\
\frac {u}{v} &= \ln\left(\frac {uT+L}{L}\right)
\end{align*}
Substituting the values given in the problem tells us 
\begin{align*}
100 = \ln\left(\frac {uT+L}{L}\right) \implies e^{100} &= \frac {uT}{L}+1 \\
 T &= \boxed{e^{100}-1}
\end{align*}
\end{solution}